removed F from RolePath. We don't need it and it is easier to explain without it

src/FcEtt/ett_ott.v
@@ -114,73 +114,6 @@ Definition theta : Set := list ( atom * pattern_arg ).
 (** subrules *)
 (** arities *)
 (** opening up abstractions *)
-Fixpoint open_brs_wrt_co_rec (k:nat) (g5:co) (brs_6:brs) {struct brs_6}: brs :=
-  match brs_6 with
-  | br_None => br_None 
-  | (br_One K a brs5) => br_One K (open_tm_wrt_co_rec k g5 a) (open_brs_wrt_co_rec k g5 brs5)
-end
-with open_tm_wrt_co_rec (k:nat) (g5:co) (a5:tm) {struct a5}: tm :=
-  match a5 with
-  | a_Star => a_Star 
-  | (a_Var_b nat) => a_Var_b nat
-  | (a_Var_f x) => a_Var_f x
-  | (a_Abs rho A b) => a_Abs rho (open_tm_wrt_co_rec k g5 A) (open_tm_wrt_co_rec k g5 b)
-  | (a_UAbs rho b) => a_UAbs rho (open_tm_wrt_co_rec k g5 b)
-  | (a_App a nu b) => a_App (open_tm_wrt_co_rec k g5 a) nu (open_tm_wrt_co_rec k g5 b)
-  | (a_Pi rho A B) => a_Pi rho (open_tm_wrt_co_rec k g5 A) (open_tm_wrt_co_rec k g5 B)
-  | (a_CAbs phi b) => a_CAbs (open_constraint_wrt_co_rec k g5 phi) (open_tm_wrt_co_rec (S k) g5 b)
-  | (a_UCAbs b) => a_UCAbs (open_tm_wrt_co_rec (S k) g5 b)
-  | (a_CApp a g) => a_CApp (open_tm_wrt_co_rec k g5 a) (open_co_wrt_co_rec k g5 g)
-  | (a_CPi phi B) => a_CPi (open_constraint_wrt_co_rec k g5 phi) (open_tm_wrt_co_rec (S k) g5 B)
-  | (a_Conv a R g) => a_Conv (open_tm_wrt_co_rec k g5 a) R (open_co_wrt_co_rec k g5 g)
-  | (a_Fam F) => a_Fam F
-  | a_Bullet => a_Bullet 
-  | (a_Pattern R a F Apps5 b1 b2) => a_Pattern R (open_tm_wrt_co_rec k g5 a) F Apps5 (open_tm_wrt_co_rec k g5 b1) (open_tm_wrt_co_rec k g5 b2)
-  | (a_DataCon K) => a_DataCon K
-  | (a_Case a brs5) => a_Case (open_tm_wrt_co_rec k g5 a) (open_brs_wrt_co_rec k g5 brs5)
-  | (a_Sub R a) => a_Sub R (open_tm_wrt_co_rec k g5 a)
-  | a_Coerce => a_Coerce 
-  | (a_SrcApp a b) => a_SrcApp (open_tm_wrt_co_rec k g5 a) (open_tm_wrt_co_rec k g5 b)
-end
-with open_constraint_wrt_co_rec (k:nat) (g5:co) (phi5:constraint) : constraint :=
-  match phi5 with
-  | (Eq a b A R) => Eq (open_tm_wrt_co_rec k g5 a) (open_tm_wrt_co_rec k g5 b) (open_tm_wrt_co_rec k g5 A) R
-end
-with open_co_wrt_co_rec (k:nat) (g_5:co) (g__6:co) {struct g__6}: co :=
-  match g__6 with
-  | g_Triv => g_Triv 
-  | (g_Var_b nat) => 
-      match lt_eq_lt_dec nat k with
-        | inleft (left _) => g_Var_b nat
-        | inleft (right _) => g_5
-        | inright _ => g_Var_b (nat - 1)
-      end
-  | (g_Var_f c) => g_Var_f c
-  | (g_Beta a b) => g_Beta (open_tm_wrt_co_rec k g_5 a) (open_tm_wrt_co_rec k g_5 b)
-  | (g_Refl a) => g_Refl (open_tm_wrt_co_rec k g_5 a)
-  | (g_Refl2 a b g) => g_Refl2 (open_tm_wrt_co_rec k g_5 a) (open_tm_wrt_co_rec k g_5 b) (open_co_wrt_co_rec k g_5 g)
-  | (g_Sym g) => g_Sym (open_co_wrt_co_rec k g_5 g)
-  | (g_Trans g1 g2) => g_Trans (open_co_wrt_co_rec k g_5 g1) (open_co_wrt_co_rec k g_5 g2)
-  | (g_Sub g) => g_Sub (open_co_wrt_co_rec k g_5 g)
-  | (g_PiCong rho R g1 g2) => g_PiCong rho R (open_co_wrt_co_rec k g_5 g1) (open_co_wrt_co_rec k g_5 g2)
-  | (g_AbsCong rho R g1 g2) => g_AbsCong rho R (open_co_wrt_co_rec k g_5 g1) (open_co_wrt_co_rec k g_5 g2)
-  | (g_AppCong g1 rho R g2) => g_AppCong (open_co_wrt_co_rec k g_5 g1) rho R (open_co_wrt_co_rec k g_5 g2)
-  | (g_PiFst g) => g_PiFst (open_co_wrt_co_rec k g_5 g)
-  | (g_CPiFst g) => g_CPiFst (open_co_wrt_co_rec k g_5 g)
-  | (g_IsoSnd g) => g_IsoSnd (open_co_wrt_co_rec k g_5 g)
-  | (g_PiSnd g1 g2) => g_PiSnd (open_co_wrt_co_rec k g_5 g1) (open_co_wrt_co_rec k g_5 g2)
-  | (g_CPiCong g1 g3) => g_CPiCong (open_co_wrt_co_rec k g_5 g1) (open_co_wrt_co_rec (S k) g_5 g3)
-  | (g_CAbsCong g1 g3 g4) => g_CAbsCong (open_co_wrt_co_rec k g_5 g1) (open_co_wrt_co_rec (S k) g_5 g3) (open_co_wrt_co_rec k g_5 g4)
-  | (g_CAppCong g g1 g2) => g_CAppCong (open_co_wrt_co_rec k g_5 g) (open_co_wrt_co_rec k g_5 g1) (open_co_wrt_co_rec k g_5 g2)
-  | (g_CPiSnd g g1 g2) => g_CPiSnd (open_co_wrt_co_rec k g_5 g) (open_co_wrt_co_rec k g_5 g1) (open_co_wrt_co_rec k g_5 g2)
-  | (g_Cast g1 R g2) => g_Cast (open_co_wrt_co_rec k g_5 g1) R (open_co_wrt_co_rec k g_5 g2)
-  | (g_EqCong g1 A g2) => g_EqCong (open_co_wrt_co_rec k g_5 g1) (open_tm_wrt_co_rec k g_5 A) (open_co_wrt_co_rec k g_5 g2)
-  | (g_IsoConv phi1 phi2 g) => g_IsoConv (open_constraint_wrt_co_rec k g_5 phi1) (open_constraint_wrt_co_rec k g_5 phi2) (open_co_wrt_co_rec k g_5 g)
-  | (g_Eta a) => g_Eta (open_tm_wrt_co_rec k g_5 a)
-  | (g_Left g g') => g_Left (open_co_wrt_co_rec k g_5 g) (open_co_wrt_co_rec k g_5 g')
-  | (g_Right g g') => g_Right (open_co_wrt_co_rec k g_5 g) (open_co_wrt_co_rec k g_5 g')
-end.
-
 Fixpoint open_brs_wrt_tm_rec (k:nat) (a5:tm) (brs_6:brs) {struct brs_6}: brs :=
   match brs_6 with
   | br_None => br_None 
@@ -248,22 +181,71 @@ with open_co_wrt_tm_rec (k:nat) (a5:tm) (g_5:co) {struct g_5}: co :=
   | (g_Right g g') => g_Right (open_co_wrt_tm_rec k a5 g) (open_co_wrt_tm_rec k a5 g')
 end.
 
-Definition open_sig_sort_wrt_co_rec (k:nat) (g5:co) (sig_sort5:sig_sort) : sig_sort :=
-  match sig_sort5 with
-  | (Cs A Rs) => Cs (open_tm_wrt_co_rec k g5 A) Rs
-  | (Ax p a A R Rs) => Ax (open_tm_wrt_co_rec k g5 p) (open_tm_wrt_co_rec k g5 a) (open_tm_wrt_co_rec k g5 A) R Rs
-end.
-
-Definition open_sig_sort_wrt_tm_rec (k:nat) (a5:tm) (sig_sort5:sig_sort) : sig_sort :=
-  match sig_sort5 with
-  | (Cs A Rs) => Cs (open_tm_wrt_tm_rec k a5 A) Rs
-  | (Ax p a A R Rs) => Ax (open_tm_wrt_tm_rec k a5 p) (open_tm_wrt_tm_rec k a5 a) (open_tm_wrt_tm_rec k a5 A) R Rs
-end.
-
-Definition open_pattern_arg_wrt_tm_rec (k:nat) (a5:tm) (pattern_arg5:pattern_arg) : pattern_arg :=
-  match pattern_arg5 with
-  | (p_Tm nu a) => p_Tm nu (open_tm_wrt_tm_rec k a5 a)
-  | (p_Co g) => p_Co (open_co_wrt_tm_rec k a5 g)
+Fixpoint open_tm_wrt_co_rec (k:nat) (g5:co) (a5:tm) {struct a5}: tm :=
+  match a5 with
+  | a_Star => a_Star 
+  | (a_Var_b nat) => a_Var_b nat
+  | (a_Var_f x) => a_Var_f x
+  | (a_Abs rho A b) => a_Abs rho (open_tm_wrt_co_rec k g5 A) (open_tm_wrt_co_rec k g5 b)
+  | (a_UAbs rho b) => a_UAbs rho (open_tm_wrt_co_rec k g5 b)
+  | (a_App a nu b) => a_App (open_tm_wrt_co_rec k g5 a) nu (open_tm_wrt_co_rec k g5 b)
+  | (a_Pi rho A B) => a_Pi rho (open_tm_wrt_co_rec k g5 A) (open_tm_wrt_co_rec k g5 B)
+  | (a_CAbs phi b) => a_CAbs (open_constraint_wrt_co_rec k g5 phi) (open_tm_wrt_co_rec (S k) g5 b)
+  | (a_UCAbs b) => a_UCAbs (open_tm_wrt_co_rec (S k) g5 b)
+  | (a_CApp a g) => a_CApp (open_tm_wrt_co_rec k g5 a) (open_co_wrt_co_rec k g5 g)
+  | (a_CPi phi B) => a_CPi (open_constraint_wrt_co_rec k g5 phi) (open_tm_wrt_co_rec (S k) g5 B)
+  | (a_Conv a R g) => a_Conv (open_tm_wrt_co_rec k g5 a) R (open_co_wrt_co_rec k g5 g)
+  | (a_Fam F) => a_Fam F
+  | a_Bullet => a_Bullet 
+  | (a_Pattern R a F Apps5 b1 b2) => a_Pattern R (open_tm_wrt_co_rec k g5 a) F Apps5 (open_tm_wrt_co_rec k g5 b1) (open_tm_wrt_co_rec k g5 b2)
+  | (a_DataCon K) => a_DataCon K
+  | (a_Case a brs5) => a_Case (open_tm_wrt_co_rec k g5 a) (open_brs_wrt_co_rec k g5 brs5)
+  | (a_Sub R a) => a_Sub R (open_tm_wrt_co_rec k g5 a)
+  | a_Coerce => a_Coerce 
+  | (a_SrcApp a b) => a_SrcApp (open_tm_wrt_co_rec k g5 a) (open_tm_wrt_co_rec k g5 b)
+end
+with open_constraint_wrt_co_rec (k:nat) (g5:co) (phi5:constraint) : constraint :=
+  match phi5 with
+  | (Eq a b A R) => Eq (open_tm_wrt_co_rec k g5 a) (open_tm_wrt_co_rec k g5 b) (open_tm_wrt_co_rec k g5 A) R
+end
+with open_co_wrt_co_rec (k:nat) (g_5:co) (g__6:co) {struct g__6}: co :=
+  match g__6 with
+  | g_Triv => g_Triv 
+  | (g_Var_b nat) => 
+      match lt_eq_lt_dec nat k with
+        | inleft (left _) => g_Var_b nat
+        | inleft (right _) => g_5
+        | inright _ => g_Var_b (nat - 1)
+      end
+  | (g_Var_f c) => g_Var_f c
+  | (g_Beta a b) => g_Beta (open_tm_wrt_co_rec k g_5 a) (open_tm_wrt_co_rec k g_5 b)
+  | (g_Refl a) => g_Refl (open_tm_wrt_co_rec k g_5 a)
+  | (g_Refl2 a b g) => g_Refl2 (open_tm_wrt_co_rec k g_5 a) (open_tm_wrt_co_rec k g_5 b) (open_co_wrt_co_rec k g_5 g)
+  | (g_Sym g) => g_Sym (open_co_wrt_co_rec k g_5 g)
+  | (g_Trans g1 g2) => g_Trans (open_co_wrt_co_rec k g_5 g1) (open_co_wrt_co_rec k g_5 g2)
+  | (g_Sub g) => g_Sub (open_co_wrt_co_rec k g_5 g)
+  | (g_PiCong rho R g1 g2) => g_PiCong rho R (open_co_wrt_co_rec k g_5 g1) (open_co_wrt_co_rec k g_5 g2)
+  | (g_AbsCong rho R g1 g2) => g_AbsCong rho R (open_co_wrt_co_rec k g_5 g1) (open_co_wrt_co_rec k g_5 g2)
+  | (g_AppCong g1 rho R g2) => g_AppCong (open_co_wrt_co_rec k g_5 g1) rho R (open_co_wrt_co_rec k g_5 g2)
+  | (g_PiFst g) => g_PiFst (open_co_wrt_co_rec k g_5 g)
+  | (g_CPiFst g) => g_CPiFst (open_co_wrt_co_rec k g_5 g)
+  | (g_IsoSnd g) => g_IsoSnd (open_co_wrt_co_rec k g_5 g)
+  | (g_PiSnd g1 g2) => g_PiSnd (open_co_wrt_co_rec k g_5 g1) (open_co_wrt_co_rec k g_5 g2)
+  | (g_CPiCong g1 g3) => g_CPiCong (open_co_wrt_co_rec k g_5 g1) (open_co_wrt_co_rec (S k) g_5 g3)
+  | (g_CAbsCong g1 g3 g4) => g_CAbsCong (open_co_wrt_co_rec k g_5 g1) (open_co_wrt_co_rec (S k) g_5 g3) (open_co_wrt_co_rec k g_5 g4)
+  | (g_CAppCong g g1 g2) => g_CAppCong (open_co_wrt_co_rec k g_5 g) (open_co_wrt_co_rec k g_5 g1) (open_co_wrt_co_rec k g_5 g2)
+  | (g_CPiSnd g g1 g2) => g_CPiSnd (open_co_wrt_co_rec k g_5 g) (open_co_wrt_co_rec k g_5 g1) (open_co_wrt_co_rec k g_5 g2)
+  | (g_Cast g1 R g2) => g_Cast (open_co_wrt_co_rec k g_5 g1) R (open_co_wrt_co_rec k g_5 g2)
+  | (g_EqCong g1 A g2) => g_EqCong (open_co_wrt_co_rec k g_5 g1) (open_tm_wrt_co_rec k g_5 A) (open_co_wrt_co_rec k g_5 g2)
+  | (g_IsoConv phi1 phi2 g) => g_IsoConv (open_constraint_wrt_co_rec k g_5 phi1) (open_constraint_wrt_co_rec k g_5 phi2) (open_co_wrt_co_rec k g_5 g)
+  | (g_Eta a) => g_Eta (open_tm_wrt_co_rec k g_5 a)
+  | (g_Left g g') => g_Left (open_co_wrt_co_rec k g_5 g) (open_co_wrt_co_rec k g_5 g')
+  | (g_Right g g') => g_Right (open_co_wrt_co_rec k g_5 g) (open_co_wrt_co_rec k g_5 g')
+end
+with open_brs_wrt_co_rec (k:nat) (g5:co) (brs_6:brs) {struct brs_6}: brs :=
+  match brs_6 with
+  | br_None => br_None 
+  | (br_One K a brs5) => br_One K (open_tm_wrt_co_rec k g5 a) (open_brs_wrt_co_rec k g5 brs5)
 end.
 
 Definition open_sort_wrt_tm_rec (k:nat) (a5:tm) (sort5:sort) : sort :=
@@ -272,10 +254,10 @@ Definition open_sort_wrt_tm_rec (k:nat) (a5:tm) (sort5:sort) : sort :=
   | (Co phi) => Co (open_constraint_wrt_tm_rec k a5 phi)
 end.
 
-Definition open_sort_wrt_co_rec (k:nat) (g5:co) (sort5:sort) : sort :=
-  match sort5 with
-  | (Tm A) => Tm (open_tm_wrt_co_rec k g5 A)
-  | (Co phi) => Co (open_constraint_wrt_co_rec k g5 phi)
+Definition open_sig_sort_wrt_tm_rec (k:nat) (a5:tm) (sig_sort5:sig_sort) : sig_sort :=
+  match sig_sort5 with
+  | (Cs A Rs) => Cs (open_tm_wrt_tm_rec k a5 A) Rs
+  | (Ax p a A R Rs) => Ax (open_tm_wrt_tm_rec k a5 p) (open_tm_wrt_tm_rec k a5 a) (open_tm_wrt_tm_rec k a5 A) R Rs
 end.
 
 Definition open_pattern_arg_wrt_co_rec (k:nat) (g5:co) (pattern_arg5:pattern_arg) : pattern_arg :=
@@ -284,33 +266,51 @@ Definition open_pattern_arg_wrt_co_rec (k:nat) (g5:co) (pattern_arg5:pattern_arg
   | (p_Co g) => p_Co (open_co_wrt_co_rec k g5 g)
 end.
 
-Definition open_brs_wrt_tm a5 brs_6 := open_brs_wrt_tm_rec 0 brs_6 a5.
+Definition open_sig_sort_wrt_co_rec (k:nat) (g5:co) (sig_sort5:sig_sort) : sig_sort :=
+  match sig_sort5 with
+  | (Cs A Rs) => Cs (open_tm_wrt_co_rec k g5 A) Rs
+  | (Ax p a A R Rs) => Ax (open_tm_wrt_co_rec k g5 p) (open_tm_wrt_co_rec k g5 a) (open_tm_wrt_co_rec k g5 A) R Rs
+end.
 
-Definition open_sig_sort_wrt_co g5 sig_sort5 := open_sig_sort_wrt_co_rec 0 sig_sort5 g5.
+Definition open_sort_wrt_co_rec (k:nat) (g5:co) (sort5:sort) : sort :=
+  match sort5 with
+  | (Tm A) => Tm (open_tm_wrt_co_rec k g5 A)
+  | (Co phi) => Co (open_constraint_wrt_co_rec k g5 phi)
+end.
 
-Definition open_sig_sort_wrt_tm a5 sig_sort5 := open_sig_sort_wrt_tm_rec 0 sig_sort5 a5.
-
-Definition open_constraint_wrt_co g5 phi5 := open_constraint_wrt_co_rec 0 phi5 g5.
+Definition open_pattern_arg_wrt_tm_rec (k:nat) (a5:tm) (pattern_arg5:pattern_arg) : pattern_arg :=
+  match pattern_arg5 with
+  | (p_Tm nu a) => p_Tm nu (open_tm_wrt_tm_rec k a5 a)
+  | (p_Co g) => p_Co (open_co_wrt_tm_rec k a5 g)
+end.
 
 Definition open_tm_wrt_co g5 a5 := open_tm_wrt_co_rec 0 a5 g5.
 
-Definition open_pattern_arg_wrt_tm a5 pattern_arg5 := open_pattern_arg_wrt_tm_rec 0 pattern_arg5 a5.
-
 Definition open_sort_wrt_tm a5 sort5 := open_sort_wrt_tm_rec 0 sort5 a5.
 
-Definition open_sort_wrt_co g5 sort5 := open_sort_wrt_co_rec 0 sort5 g5.
-
-Definition open_brs_wrt_co g5 brs_6 := open_brs_wrt_co_rec 0 brs_6 g5.
+Definition open_sig_sort_wrt_tm a5 sig_sort5 := open_sig_sort_wrt_tm_rec 0 sig_sort5 a5.
 
 Definition open_constraint_wrt_tm a5 phi5 := open_constraint_wrt_tm_rec 0 phi5 a5.
 
-Definition open_co_wrt_co g_5 g__6 := open_co_wrt_co_rec 0 g__6 g_5.
+Definition open_tm_wrt_tm a5 a_6 := open_tm_wrt_tm_rec 0 a_6 a5.
 
-Definition open_co_wrt_tm a5 g_5 := open_co_wrt_tm_rec 0 g_5 a5.
+Definition open_brs_wrt_tm a5 brs_6 := open_brs_wrt_tm_rec 0 brs_6 a5.
 
 Definition open_pattern_arg_wrt_co g5 pattern_arg5 := open_pattern_arg_wrt_co_rec 0 pattern_arg5 g5.
 
-Definition open_tm_wrt_tm a5 a_6 := open_tm_wrt_tm_rec 0 a_6 a5.
+Definition open_co_wrt_tm a5 g_5 := open_co_wrt_tm_rec 0 g_5 a5.
+
+Definition open_brs_wrt_co g5 brs_6 := open_brs_wrt_co_rec 0 brs_6 g5.
+
+Definition open_sig_sort_wrt_co g5 sig_sort5 := open_sig_sort_wrt_co_rec 0 sig_sort5 g5.
+
+Definition open_sort_wrt_co g5 sort5 := open_sort_wrt_co_rec 0 sort5 g5.
+
+Definition open_pattern_arg_wrt_tm a5 pattern_arg5 := open_pattern_arg_wrt_tm_rec 0 pattern_arg5 a5.
+
+Definition open_co_wrt_co g_5 g__6 := open_co_wrt_co_rec 0 g__6 g_5.
+
+Definition open_constraint_wrt_co g5 phi5 := open_constraint_wrt_co_rec 0 phi5 g5.
 
 (** terms are locally-closed pre-terms *)
 (** definitions *)
@@ -1053,27 +1053,27 @@ Inductive SubRole : role -> role -> Prop :=    (* defn SubRole *)
      SubRole R1 R3.
 
 (* defns JRolePath *)
-Inductive RolePath : tm -> const -> roles -> Prop :=    (* defn RolePath *)
+Inductive RolePath : tm -> roles -> Prop :=    (* defn RolePath *)
  | RolePath_AbsConst : forall (F:const) (Rs:roles) (A:tm),
       binds  F  ( (Cs A Rs) )   toplevel   ->
-     RolePath (a_Fam F) F Rs
+     RolePath (a_Fam F) Rs
  | RolePath_Const : forall (F:const) (Rs:roles) (p a A:tm) (R1:role),
       binds  F  ( (Ax p a A R1 Rs) )   toplevel   ->
-     RolePath (a_Fam F) F Rs
- | RolePath_TApp : forall (a:tm) (R1:role) (b':tm) (F:const) (Rs:roles),
-     lc_tm b' ->
-     RolePath a F  ( R1 :: Rs )  ->
-     RolePath  ( (a_App a (Role R1) b') )  F Rs
- | RolePath_App : forall (a b':tm) (F:const) (Rs:roles),
-     lc_tm b' ->
-     RolePath a F  ( Nom :: Rs )  ->
-     RolePath  ( (a_App a (Rho Rel) b') )  F Rs
- | RolePath_IApp : forall (a:tm) (F:const) (Rs:roles),
-     RolePath a F Rs ->
-     RolePath  ( (a_App a (Rho Irrel) a_Bullet) )  F Rs
- | RolePath_CApp : forall (a:tm) (F:const) (Rs:roles),
-     RolePath a F Rs ->
-     RolePath  ( (a_CApp a g_Triv) )  F Rs.
+     RolePath (a_Fam F) Rs
+ | RolePath_TApp : forall (a:tm) (R1:role) (b:tm) (Rs:roles),
+     lc_tm b ->
+     RolePath a  ( R1 :: Rs )  ->
+     RolePath (a_App a (Role R1) b) Rs
+ | RolePath_App : forall (a b:tm) (Rs:roles),
+     lc_tm b ->
+     RolePath a  ( Nom :: Rs )  ->
+     RolePath (a_App a (Rho Rel) b) Rs
+ | RolePath_IApp : forall (a:tm) (Rs:roles),
+     RolePath a Rs ->
+     RolePath (a_App a (Rho Irrel) a_Bullet) Rs
+ | RolePath_CApp : forall (a:tm) (Rs:roles),
+     RolePath a Rs ->
+     RolePath (a_CApp a g_Triv) Rs.
 
 (* defns JAppsPath *)
 Inductive AppsPath : role -> tm -> const -> Apps -> Prop :=    (* defn AppsPath *)
@@ -1634,10 +1634,10 @@ with Typing : context -> tm -> tm -> Prop :=    (* defn Typing *)
      Typing G b (a_Pi Rel A B) ->
      Typing G a A ->
      Typing G (a_App b (Rho Rel) a)  (open_tm_wrt_tm  B   a ) 
- | E_TApp : forall (G:context) (b:tm) (R:role) (a B A:tm) (F:const) (Rs:roles),
+ | E_TApp : forall (G:context) (b:tm) (R:role) (a B A:tm) (Rs:roles),
      Typing G b (a_Pi Rel A B) ->
      Typing G a A ->
-     RolePath b F  ( R :: Rs )  ->
+     RolePath b  ( R :: Rs )  ->
      Typing G (a_App b (Role R) a)  (open_tm_wrt_tm  B   a ) 
  | E_IApp : forall (G:context) (b B a A:tm),
      Typing G b (a_Pi Irrel A B) ->
@@ -1733,11 +1733,11 @@ with DefEq : context -> available_props -> tm -> tm -> tm -> role -> Prop :=    
      DefEq G D a1 b1  ( (a_Pi Rel A B) )  R' ->
      DefEq G D a2 b2 A Nom ->
      DefEq G D (a_App a1 (Rho Rel) a2) (a_App b1 (Rho Rel) b2)  (  (open_tm_wrt_tm  B   a2 )  )  R'
- | E_TAppCong : forall (G:context) (D:available_props) (a1:tm) (R:role) (a2 b1 b2 B:tm) (R':role) (A:tm) (F:const) (Rs:roles),
+ | E_TAppCong : forall (G:context) (D:available_props) (a1:tm) (R:role) (a2 b1 b2 B:tm) (R':role) (A:tm) (Rs:roles),
      DefEq G D a1 b1  ( (a_Pi Rel A B) )  R' ->
      DefEq G D a2 b2 A  (param R   R' )  ->
-     RolePath a1 F  ( R :: Rs )  ->
-     RolePath b1 F  ( R :: Rs )  ->
+     RolePath a1  ( R :: Rs )  ->
+     RolePath b1  ( R :: Rs )  ->
      Typing G (a_App b1 (Role R) b2)  (open_tm_wrt_tm  B   a2 )  ->
      DefEq G D (a_App a1 (Role R) a2) (a_App b1 (Role R) b2)  (  (open_tm_wrt_tm  B   a2 )  )  R'
  | E_IAppCong : forall (G:context) (D:available_props) (a1 b1 B a:tm) (R':role) (A:tm),
@@ -1990,10 +1990,10 @@ with SrcTrans : context -> tm -> tm -> tm -> Prop :=    (* defn SrcTrans *)
      SrcTrans G b b' (a_Pi Rel A B) ->
      SrcTrans G a a' A ->
      SrcTrans G (a_SrcApp b a) (a_App b' (Rho Rel) a')  (open_tm_wrt_tm  B   a' ) 
- | ST_TApp : forall (G:context) (b a b':tm) (R:role) (a' B A:tm) (F:const) (Rs:roles),
+ | ST_TApp : forall (G:context) (b a b':tm) (R:role) (a' B A:tm) (Rs:roles),
      SrcTrans G b b' (a_Pi Rel A B) ->
      SrcTrans G a a' A ->
-     RolePath b F  ( R :: Rs )  ->
+     RolePath b  ( R :: Rs )  ->
      SrcTrans G (a_SrcApp b a) (a_App b' (Role R) a')  (open_tm_wrt_tm  B   a ) 
  | ST_IApp : forall (G:context) (b b' B a A:tm),
      SrcTrans G b b' (a_Pi Irrel A B) ->
